concurrency/openmp_sem/reduction.v
@@ -1,18 +1,18 @@
 From Coq Require Import String ZArith.
-From compcert Require Import Clight Cop Clightdefs AST Integers Ctypes.
+From compcert Require Import Clight Cop Clightdefs AST Integers Ctypes Values.
+From compcert Require Import -(notations) lib.Maps.
+From VST.concurrency.openmp_sem Require Import notations.
+From RecordUpdate Require Import RecordSet.
+Import RecordSetNotations.
 
-From stdpp Require Import base decidable.
+(* From VST.concurrency.openmp_sem Require Import notations.  *)
+From stdpp Require Import base list.
 
-(* same as in Clightdefs, just redefine notation *)
-Notation "$$ s" := (ltac:(ClightNotations.ident_of_string s))
-                  (at level 1, only parsing) : clight_scope.
-
-Local Open Scope string_scope.
-Local Open Scope clight_scope.
-Definition __max : ident := $$"max".
-Definition __min : ident := $$"min".
-
-(* mathematical value of a privatized reduction variable
+(* This is not used directly, only serves as a reference.
+   Mathematical value of a privatized reduction variable
+   We need the initial value to be injected in compcert val type, and we obtain that by
+   evaluating an initializer expression in the executing environment and memory.
+   
    [Standard 6.0, Table 7.1: (Initializer for) Implicitly Declared C/C++ Reduction Identifiers]  *)
     Definition reduction_var_init_val (i: reduction_identifier_type) : option nat :=
         match i with
@@ -88,3 +88,67 @@ Definition __min : ident := $$"min".
 (* Standard 6.0, 7.6.2.1: "The number of times that the combiner expression is executed and the
    order of these executions for any reduction clause are unspecified."
 *)
+
+    
+    (* maps of ident -> original val, list of a thread's final contribution to the privatized var,
+       where i is originated from the global / local / temporal env. *)
+    Record privatized_vars :=
+      { in_ge: PTree.t $ (val * list val)%type;
+     (* in_le: PTree.t $ (val * list val)%type; *)
+        in_te: PTree.t $ (val * list val)%type }.
+
+    #[export] Instance settable_ot_info : Settable _ := settable! Build_privatized_vars <in_ge; in_te>.
+
+    (* assume that the ident is not already in pv *)
+    Definition add_privatized_te (i: ident) (orig: val) (pv: privatized_vars) : option privatized_vars :=
+        match pv.(in_te) ! i with
+        | None => Some $ pv <| in_te ::= PTree.set i (orig, nil) |>
+        | _ => None
+        end.
+
+    (* the initial value for reduction operation `red_id_type` and ctype `ty` is `v` *)
+    Inductive init_val_rel ge e te m red_id_type ty v : Prop :=
+    | InitVal:
+        ∀ init_expr,
+        initializer_expr red_id_type ty init_expr ->
+        eval_expr ge e te m init_expr v ->
+        init_val_rel ge e te m red_id_type ty v.
+
+    (* information about one variable being reduced *)
+    Record red_witness :=
+        {
+            red_ident: reduction_identifier_type;
+            red_var: red_var_type;
+            init_val: val
+        }.
+    #[export] Instance settable_red_witness : Settable _ := settable! Build_red_witness <red_ident; red_var; init_val>.
+        
+    (* add a reduction variable to the privatized_vars, set initial value for temp_env *)
+    Definition add_red_var (wit: red_witness) pv te
+                           : option (privatized_vars * temp_env) :=
+        let red_name := wit.(red_var).(red_var_name) in
+        let init_val := wit.(init_val) in
+        match wit.(red_var).(red_var_scope) with
+        | VarScopeGlobal => None (* TODO *)
+        | VarScopeLocal  => None (* with the builtin reduction operators, reducing for lvalues are unsupported *)
+        | VarScopeTemp   => v ← (te ! red_name);
+                            pv' ← add_privatized_te red_name v pv;
+                            Some (pv', PTree.set red_name init_val te)
+        end.
+
+    (* add a list of reduction variables to pv and set up temp_env *)
+    Definition add_red_clause (wits: list red_witness) pv te : option (privatized_vars * temp_env) :=
+            foldr (λ wit acc, pv_te ← acc; let '(pv, te) := pv_te in add_red_var wit pv te) (Some (pv, te)) wits
+    .
+
+    (* wits holds the initial values for the reduction variables in the clause, and these values are the results of
+       evaluating the initializing expressions under current envs and mem *)
+    Inductive wits_for_red_clause ge e te m (rc: reduction_clause_type) (wits: list red_witness) : Prop :=
+    | WitsForRedClause:
+        match rc with
+        | RedClause red_id_type red_vars =>
+            Forall2 (λ rv wit, init_val_rel ge e te m red_id_type rv.(red_var_c_type) wit.(init_val)) red_vars wits
+        end ->
+        wits_for_red_clause ge e te m rc wits.
+
+    (* the reduction clause is a list of reduction variables, each with an initializer expression *)
